InferenceInLean/Exercises.lean
@@ -8,13 +8,13 @@ open FirstOrder
 -/
 
 inductive PeanoFuns where
-    | zero
-    | succ
-    | add
-    | mul
+  | zero
+  | succ
+  | add
+  | mul
 
 inductive PeanoPreds where
-    | less_than
+  | less_than
 
 @[simp]
 def ex_sig_peano : Signature := ⟨PeanoFuns, PeanoPreds⟩
@@ -24,54 +24,51 @@ def ex_sig_peano : Signature := ⟨PeanoFuns, PeanoPreds⟩
 -/
 @[simp]
 def ex_formula_peano : @Formula ex_sig_peano String :=
-    .all "x" (.all "y" (.iff
-        (.or
-            (.atom (.pred .less_than [.var "x", .var "y"]))
-            (.atom (.eq (.var "x") (.var "y")))
-        )
-        (.ex "z"
-            (.atom (.eq (.func .add [.var "x", .var "z"]) (.var "y")))
-        )
-    ))
+  .all "x" <| .all "y" <| .iff
+    (.or
+      (.atom (.pred .less_than [.var "x", .var "y"]))
+      (.atom (.eq (.var "x") (.var "y"))))
+    (.ex "z" (.atom (.eq (.func .add [.var "x", .var "z"]) (.var "y"))))
 
 @[simp]
-def ex_interpret_peano : Interpretation ex_sig_peano :=
-    {
-      univ := ℕ
-      functions := λ
-        | .zero => λ _ => 0
-        | .succ => λ xs => xs[0]! + 1
-        | .add => λ xs => xs[0]! + xs[1]!
-        | .mul => λ xs => xs[0]! * xs[1]!
-      predicates := λ f => match f with
-        | .less_than => λ xs => xs[0]! < xs[1]!
-    }
+def ex_interpret_peano : Interpretation ex_sig_peano where
+  univ := ℕ
+  functions := λ
+    | .zero => λ _ => 0
+    | .succ => λ xs => xs[0]! + 1
+    | .add => λ xs => xs[0]! + xs[1]!
+    | .mul => λ xs => xs[0]! * xs[1]!
+  predicates := λ f => match f with
+    | .less_than => λ xs => xs[0]! < xs[1]!
 
 def ex_assig_peano : Assignment String Nat
-    | "x" => 0
-    | "y" => 0
-    | _ => 0
+  | "x" => 0
+  | "y" => 0
+  | _ => 0
 
 def example_substitution : Substitution ex_sig_peano String := λ x => match x with
-    | "x" => Term.func .succ [Term.var "y"]
-    | _ => Term.var x
+  | "x" => Term.func .succ [Term.var "y"]
+  | _ => Term.var x
 
 def ex_formula_peano_lt : @Formula ex_sig_peano String :=
-    .all "z" (.atom $ .pred .less_than [.var "x", .func .succ [.func .succ [.var "z"]]])
+  .all "z" (.atom $ .pred .less_than [.var "x", .func .succ [.func .succ [.var "z"]]])
 
-lemma ex_proof_lt : @Formula.eval ex_sig_peano String (@instBEqOfDecidableEq String instDecidableEqString)
+lemma ex_proof_lt : @Formula.eval ex_sig_peano String
+    (@instBEqOfDecidableEq String instDecidableEqString)
     ex_interpret_peano ex_assig_peano ex_formula_peano_lt := by
-        simp [ex_formula_peano_lt, ex_sig_peano, Interpretation, Assignment, ex_assig_peano]
+  simp [ex_formula_peano_lt, ex_sig_peano, Interpretation, Assignment, ex_assig_peano]
 
-noncomputable def ex_formula_peano_lt_subst : @Formula ex_sig_peano String := ex_formula_peano_lt.substitute example_substitution
+noncomputable def ex_formula_peano_lt_subst : @Formula ex_sig_peano String :=
+  ex_formula_peano_lt.substitute example_substitution
 
-lemma ex_proof_lt_subst : @Formula.eval ex_sig_peano String (@instBEqOfDecidableEq String instDecidableEqString)
+lemma ex_proof_lt_subst : @Formula.eval ex_sig_peano String
+    (@instBEqOfDecidableEq String instDecidableEqString)
     ex_interpret_peano ex_assig_peano ex_formula_peano_lt_subst := by
-        simp only [ex_sig_peano, ex_interpret_peano, ex_formula_peano_lt_subst]
-        unfold example_substitution
-        simp only [example_substitution, ex_sig_peano]
-        rw [ex_formula_peano_lt]
-        simp [Formula.substitute, ex_interpret_peano, ex_assig_peano]
+  simp only [ex_sig_peano, ex_interpret_peano, ex_formula_peano_lt_subst]
+  unfold example_substitution
+  simp only [example_substitution, ex_sig_peano]
+  rw [ex_formula_peano_lt]
+  simp [Formula.substitute, ex_interpret_peano, ex_assig_peano]
 
 #eval @Term.eval ex_sig_peano String ex_interpret_peano ex_assig_peano (Term.var "y")
 
@@ -80,29 +77,32 @@ def ex_term_peano : Term ex_sig_peano String :=
 
 #eval @Term.eval ex_sig_peano String ex_interpret_peano ex_assig_peano ex_term_peano
 
-lemma ex_peano_proof: @Formula.eval ex_sig_peano String (@instBEqOfDecidableEq String instDecidableEqString) ex_interpret_peano ex_assig_peano ex_formula_peano := by
-    simp
-    intro a b
-    apply Iff.intro
-    · intro h
-      cases h
-      next h' => use b - a
-                 refine Nat.add_sub_of_le ?_
-                 exact h'.le
-      · use 0; assumption
-    · intro h
-      obtain ⟨z, hz⟩ := h
-      cases hz
-      simp only [Nat.lt_add_right_iff_pos, Nat.self_eq_add_right]
-      exact Or.symm (Nat.eq_zero_or_pos z)
+lemma ex_peano_proof: @Formula.eval ex_sig_peano String
+    (@instBEqOfDecidableEq String instDecidableEqString)
+    ex_interpret_peano ex_assig_peano ex_formula_peano := by
+  simp
+  intro a b
+  apply Iff.intro
+  · intro h
+    cases h
+    next h' =>
+      use b - a
+      refine Nat.add_sub_of_le ?_
+      exact h'.le
+    · use 0; assumption
+  · intro h
+    obtain ⟨z, hz⟩ := h
+    cases hz
+    simp only [Nat.lt_add_right_iff_pos, Nat.self_eq_add_right]
+    exact Or.symm (Nat.eq_zero_or_pos z)
 
 def exa : Formula ex_sig_peano String := .and .falsum .verum
 example : ¬@Formula.eval ex_sig_peano _ _ ex_interpret_peano ex_assig_peano exa :=
-    of_eq_true (Eq.trans (congrArg Not (and_true False)) not_false_eq_true)
+  of_eq_true (Eq.trans (congrArg Not (and_true False)) not_false_eq_true)
 
 
 example : @EntailsInterpret ex_sig_peano String _ ex_interpret_peano
-            ex_assig_peano ex_formula_peano := ex_peano_proof
+  ex_assig_peano ex_formula_peano := ex_peano_proof
 
 
 /-
@@ -110,25 +110,21 @@ Proposition 3.3.3 Let F and G be formulas, let N be a set of formulas. Then
 (i) F is valid if and only if ¬F is unsatisfiable.
 (ii) F |= G if and only if F ∧ ¬G is unsatisfiable.
 -/
-theorem valid_iff_not_unsat
-    {sig : Signature} {X : Variables} [inst : BEq X] (F : Formula sig X) :
-    Valid F ↔ @Unsatisfiable sig X inst (Formula.neg F) := by
-        simp
+theorem valid_iff_not_unsat {sig : Signature} {X : Variables} [inst : BEq X] (F : Formula sig X) :
+    Valid F ↔ @Unsatisfiable sig X inst (Formula.neg F) := by simp
 
-theorem entails_iff_and_not_unsat
-    {sig : Signature} {X : Variables} [inst : BEq X] (F G : Formula sig X) :
-    Entails F G ↔ @Unsatisfiable sig X inst (Formula.and F (Formula.neg G)) := by
-        simp
+theorem entails_iff_and_not_unsat {sig : Signature} {X : Variables} [inst : BEq X]
+    (F G : Formula sig X) :
+    Entails F G ↔ @Unsatisfiable sig X inst (Formula.and F (Formula.neg G)) := by simp
 
 /-
 -- TODO: finish this proof
 (iii) N |= G if and only if N ∪ {¬G} is unsatisfiable.
 -/
-theorem setEntails_iff_union_not_unsat
-    {sig : Signature} {X : Variables} [inst : BEq X] (N : Set $ Formula sig X) (G : Formula sig X) :
+theorem setEntails_iff_union_not_unsat {sig : Signature} {X : Variables} [inst : BEq X]
+    (N : Set $ Formula sig X) (G : Formula sig X) :
     SetEntails N G ↔ @SetUnsatisfiable sig X inst (N ∪ {Formula.neg G}) := by
         sorry
-
 
 /-
 Exercise 4.7 (*)
@@ -143,29 +139,29 @@ theorem ex_4_7 {sig : Signature} {X : Variables} [BEq X]
     (hSnoCompl : ∀ L ∈ S, L.comp ∉ S)
     (hNsatByS : ∀ C ∈ N, ∃ L ∈ C, L ∈ S) (hN'noComplS : ∀ C ∈ N', ∀ L ∈ C, L ∉ S) :
     (ClauseSetSatisfiable (N ∪ N') ↔ ClauseSetSatisfiable N') := by
-        apply Iff.intro
-        · simp [ClauseSetSatisfiable]
-          intro I β
-          intro h
-          apply Exists.intro
-          · apply Exists.intro
-            · intro C a
-              apply h
-              simp_all only [or_true]
-        · simp [ClauseSetSatisfiable]
-          intro I_N' β_N'
-          intro hN'sat
-          use I_N'
-          use β_N'
-          intro C hC
-          cases hC
-          /- This is the actual hard case of this exercise. On paper it might look like this:
-             - Show that I_N' and β_N' do not contradict (SAT N) (this is due to hN'noComplS)
-             - Expand β_N' by the assignments implied by S to β_N'andS
-             - then β_N'andS satisfies N using hNsatByS
-          -/
-          next h => sorry
-          next h => exact hN'sat C h
+  apply Iff.intro
+  · simp [ClauseSetSatisfiable]
+    intro I β
+    intro h
+    apply Exists.intro
+    · apply Exists.intro
+      · intro C a
+        apply h
+        simp_all only [or_true]
+  · simp [ClauseSetSatisfiable]
+    intro I_N' β_N'
+    intro hN'sat
+    use I_N'
+    use β_N'
+    intro C hC
+    cases hC
+    /- This is the actual hard case of this exercise. On paper it might look like this:
+        - Show that I_N' and β_N' do not contradict (SAT N) (this is due to hN'noComplS)
+        - Expand β_N' by the assignments implied by S to β_N'andS
+        - then β_N'andS satisfies N using hNsatByS
+    -/
+    next h => sorry
+    next h => exact hN'sat C h
 
 
 lemma test {M : Set ℕ} (h : ∀ a, a ∉ M): M = ∅ := by exact Set.eq_empty_of_forall_not_mem h
